theories/rea_designs/utp_rdes_prog.thy
@@ -1,6 +1,46 @@
+section \<open> Reactive Design Programs \<close>
+
 theory utp_rdes_prog
-  imports utp_rdes_normal
+  imports 
+    utp_rdes_normal
+    utp_rdes_tactics
+    utp_rdes_parallel
 begin
+
+subsection \<open> State substitution \<close>
+
+lemma srd_subst_RHS_tri_design [usubst]:
+  "\<lceil>\<sigma>\<rceil>\<^sub>S\<^sub>\<sigma> \<dagger> \<^bold>R\<^sub>s(P \<turnstile> Q \<diamondop> R) = \<^bold>R\<^sub>s((\<lceil>\<sigma>\<rceil>\<^sub>S\<^sub>\<sigma> \<dagger> P) \<turnstile> (\<lceil>\<sigma>\<rceil>\<^sub>S\<^sub>\<sigma> \<dagger> Q) \<diamondop> (\<lceil>\<sigma>\<rceil>\<^sub>S\<^sub>\<sigma> \<dagger> R))"
+  by (rel_auto)
+
+lemma srd_subst_SRD_closed [closure]: 
+  assumes "P is SRD"
+  shows "\<lceil>\<sigma>\<rceil>\<^sub>S\<^sub>\<sigma> \<dagger> P is SRD"
+proof -
+  have "SRD(\<lceil>\<sigma>\<rceil>\<^sub>S\<^sub>\<sigma> \<dagger> (SRD P)) = \<lceil>\<sigma>\<rceil>\<^sub>S\<^sub>\<sigma> \<dagger> (SRD P)"
+    by (rel_auto)
+  thus ?thesis
+    by (metis Healthy_def assms)
+qed
+
+lemma preR_srd_subst [rdes]:
+  "pre\<^sub>R(\<lceil>\<sigma>\<rceil>\<^sub>S\<^sub>\<sigma> \<dagger> P) = \<lceil>\<sigma>\<rceil>\<^sub>S\<^sub>\<sigma> \<dagger> pre\<^sub>R(P)"
+  by (rel_auto)
+
+lemma periR_srd_subst [rdes]:
+  "peri\<^sub>R(\<lceil>\<sigma>\<rceil>\<^sub>S\<^sub>\<sigma> \<dagger> P) = \<lceil>\<sigma>\<rceil>\<^sub>S\<^sub>\<sigma> \<dagger> peri\<^sub>R(P)"
+  by (rel_auto)
+
+lemma postR_srd_subst [rdes]:
+  "post\<^sub>R(\<lceil>\<sigma>\<rceil>\<^sub>S\<^sub>\<sigma> \<dagger> P) = \<lceil>\<sigma>\<rceil>\<^sub>S\<^sub>\<sigma> \<dagger> post\<^sub>R(P)"
+  by (rel_auto)
+
+lemma srd_subst_NSRD_closed [closure]: 
+  assumes "P is NSRD"
+  shows "\<lceil>\<sigma>\<rceil>\<^sub>S\<^sub>\<sigma> \<dagger> P is NSRD"
+  by (rule NSRD_RC_intro, simp_all add: closure rdes assms unrest)
+
+subsection \<open> Assignment \<close>
 
 definition assigns_srd :: "'s usubst \<Rightarrow> ('s, 't::trace, '\<alpha>) hrel_rsp" ("\<langle>_\<rangle>\<^sub>R") where
 [upred_defs]: "assigns_srd \<sigma> = \<^bold>R\<^sub>s(true \<turnstile> ($tr\<acute> =\<^sub>u $tr \<and> \<not> $wait\<acute> \<and> \<lceil>\<langle>\<sigma>\<rangle>\<^sub>a\<rceil>\<^sub>S \<and> $\<Sigma>\<^sub>S\<acute> =\<^sub>u $\<Sigma>\<^sub>S))"
@@ -15,9 +55,127 @@ translations
   "_assign_srd x v" <= "_assign_srd (_spvar x) v"
   "x,y :=\<^sub>R u,v" <= "CONST assigns_srd (CONST subst_upd (CONST subst_upd (CONST id) (CONST svar x) u) (CONST svar y) v)"
 
+lemma assigns_srd_RHS_tri_des [rdes_def]:
+  "\<langle>\<sigma>\<rangle>\<^sub>R = \<^bold>R\<^sub>s(true\<^sub>r \<turnstile> false \<diamondop> \<langle>\<sigma>\<rangle>\<^sub>r)"
+  by (rel_auto)
+
+lemma assigns_srd_NSRD_closed [closure]: "\<langle>\<sigma>\<rangle>\<^sub>R is NSRD"
+  by (simp add: rdes_def closure unrest)
+
+lemma preR_assigns_srd [rdes]: "pre\<^sub>R(\<langle>\<sigma>\<rangle>\<^sub>R) = true\<^sub>r"
+  by (simp add: rdes_def rdes closure)
+    
+lemma periR_assigns_srd [rdes]: "peri\<^sub>R(\<langle>\<sigma>\<rangle>\<^sub>R) = false"
+  by (simp add: rdes_def rdes closure)
+
+lemma postR_assigns_srd [rdes]: "post\<^sub>R(\<langle>\<sigma>\<rangle>\<^sub>R) = \<langle>\<sigma>\<rangle>\<^sub>r"
+  by (simp add: rdes_def rdes closure rpred)
+
+subsection \<open> Conditional \<close>
+
+lemma preR_cond_srea [rdes]:
+  "pre\<^sub>R(P \<triangleleft> b \<triangleright>\<^sub>R Q) = ([b]\<^sub>S\<^sub>< \<and> pre\<^sub>R(P) \<or> [\<not>b]\<^sub>S\<^sub>< \<and> pre\<^sub>R(Q))"
+  by (rel_auto)
+
+lemma periR_cond_srea [rdes]:
+  assumes "P is SRD" "Q is SRD"
+  shows "peri\<^sub>R(P \<triangleleft> b \<triangleright>\<^sub>R Q) = ([b]\<^sub>S\<^sub>< \<and> peri\<^sub>R(P) \<or> [\<not>b]\<^sub>S\<^sub>< \<and> peri\<^sub>R(Q))"
+proof -
+  have "peri\<^sub>R(P \<triangleleft> b \<triangleright>\<^sub>R Q) = peri\<^sub>R(R1(P) \<triangleleft> b \<triangleright>\<^sub>R R1(Q))"
+    by (simp add: Healthy_if SRD_healths assms)
+  thus ?thesis
+    by (rel_auto)
+qed
+
+lemma postR_cond_srea [rdes]:
+  assumes "P is SRD" "Q is SRD"
+  shows "post\<^sub>R(P \<triangleleft> b \<triangleright>\<^sub>R Q) = ([b]\<^sub>S\<^sub>< \<and> post\<^sub>R(P) \<or> [\<not>b]\<^sub>S\<^sub>< \<and> post\<^sub>R(Q))"
+proof -
+  have "post\<^sub>R(P \<triangleleft> b \<triangleright>\<^sub>R Q) = post\<^sub>R(R1(P) \<triangleleft> b \<triangleright>\<^sub>R R1(Q))"
+    by (simp add: Healthy_if SRD_healths assms)
+  thus ?thesis
+    by (rel_auto)
+qed
+
+lemma NSRD_cond_srea [closure]:
+  assumes "P is NSRD" "Q is NSRD"
+  shows "P \<triangleleft> b \<triangleright>\<^sub>R Q is NSRD"
+proof (rule NSRD_RC_intro)
+  show "P \<triangleleft> b \<triangleright>\<^sub>R Q is SRD"
+    by (simp add: closure assms)
+  show "pre\<^sub>R (P \<triangleleft> b \<triangleright>\<^sub>R Q) is RC"
+  proof -
+    have 1:"(\<lceil>\<not> b\<rceil>\<^sub>S\<^sub>< \<or> \<not>\<^sub>r pre\<^sub>R P) ;; R1(true) = (\<lceil>\<not> b\<rceil>\<^sub>S\<^sub>< \<or> \<not>\<^sub>r pre\<^sub>R P)"
+      by (metis (no_types, lifting) NSRD_neg_pre_unit aext_not assms(1) seqr_or_distl st_lift_R1_true_right)
+    have 2:"(\<lceil>b\<rceil>\<^sub>S\<^sub>< \<or> \<not>\<^sub>r pre\<^sub>R Q) ;; R1(true) = (\<lceil>b\<rceil>\<^sub>S\<^sub>< \<or> \<not>\<^sub>r pre\<^sub>R Q)"
+      by (simp add: NSRD_neg_pre_unit assms seqr_or_distl st_lift_R1_true_right)
+    show ?thesis
+      by (simp add: rdes closure assms)
+  qed
+  show "$st\<acute> \<sharp> peri\<^sub>R (P \<triangleleft> b \<triangleright>\<^sub>R Q)"
+   by (simp add: rdes assms closure unrest)
+qed
+
+subsection \<open> Alternation \<close>
+  
+definition AlternateR 
+  :: "'a set \<Rightarrow> ('a \<Rightarrow> 's upred) \<Rightarrow> ('a \<Rightarrow> ('s, 't::trace, '\<alpha>) hrel_rsp) \<Rightarrow> ('s, 't, '\<alpha>) hrel_rsp" where
+[upred_defs]:
+"AlternateR A g P = \<^bold>R\<^sub>s(((\<Or> i\<in>A \<bullet> [g(i)]\<^sub>S\<^sub><) \<and> (\<And> i\<in>A \<bullet> [g(i)]\<^sub>S\<^sub>< \<Rightarrow>\<^sub>r pre\<^sub>R(P i))) 
+                       \<turnstile> (\<Or> i\<in>A \<bullet> [g(i)]\<^sub>S\<^sub>< \<and> peri\<^sub>R(P i)) 
+                       \<diamondop> (\<Or> i\<in>A \<bullet> [g(i)]\<^sub>S\<^sub>< \<and> post\<^sub>R(P i)))"
+
+syntax
+  "_altind_srd" :: "pttrn \<Rightarrow> logic \<Rightarrow> logic \<Rightarrow> logic \<Rightarrow> logic" ("if\<^sub>R _\<in>_ \<bullet> _ \<rightarrow> _ fi")
+  
+translations
+  "_altind_srd x A g P" => "CONST AlternateR A (\<lambda> x. g) (\<lambda> x. P)"
+  "_altind_srd x A g P" <= "CONST AlternateR A (\<lambda> x. g) (\<lambda> x'. P)"
+  
+lemma AlternateR_NSRD_closed: 
+  assumes "\<And> i. P(i) is NSRD"
+  shows "AlternateR A g P is NSRD"
+proof (cases "A = {}")
+  case True
+  then show ?thesis 
+    by (simp add: AlternateR_def closure unrest) 
+next
+  case False
+  then show ?thesis
+    by (simp add: AlternateR_def closure unrest assms)
+qed
+  
+lemma AlternateR_rdes_def [rdes_def]: 
+  assumes "\<And> i. P\<^sub>1(i) is RR" "\<And> i. P\<^sub>2(i) is RR" "\<And> i. P\<^sub>3(i) is RR"
+  shows
+  "if\<^sub>R i \<in> A \<bullet> g(i) \<rightarrow> \<^bold>R\<^sub>s(P\<^sub>1(i) \<turnstile> P\<^sub>2(i) \<diamondop> P\<^sub>3(i)) fi = 
+    \<^bold>R\<^sub>s(((\<Or> i\<in>A \<bullet> [g(i)]\<^sub>S\<^sub><) \<and> (\<And> i\<in>A \<bullet> [g(i)]\<^sub>S\<^sub>< \<Rightarrow>\<^sub>r P\<^sub>1 i)) 
+        \<turnstile> (\<Or> i\<in>A \<bullet> [g(i)]\<^sub>S\<^sub>< \<and> P\<^sub>2 i) 
+        \<diamondop> (\<Or> i\<in>A \<bullet> [g(i)]\<^sub>S\<^sub>< \<and> P\<^sub>3 i))"
+  by (simp add: AlternateR_def rdes closure assms, rel_auto)
+
+subsection \<open> Choose \<close>
+
 definition choose_srd :: "('s,'t::trace,'\<alpha>) hrel_rsp" ("choose\<^sub>R") where
 [upred_defs, rdes_def]: "choose\<^sub>R = \<^bold>R\<^sub>s(true\<^sub>r \<turnstile> false \<diamondop> true\<^sub>r)"
   
+lemma preR_choose [rdes]: "pre\<^sub>R(choose\<^sub>R) = true\<^sub>r"
+  by (rel_auto)
+
+lemma periR_choose [rdes]: "peri\<^sub>R(choose\<^sub>R) = false"
+  by (rel_auto)
+
+lemma postR_choose [rdes]: "post\<^sub>R(choose\<^sub>R) = true\<^sub>r"
+  by (rel_auto)
+    
+lemma choose_srd_SRD [closure]: "choose\<^sub>R is SRD"
+  by (simp add: choose_srd_def closure unrest)
+
+lemma NSRD_choose_srd [closure]: "choose\<^sub>R is NSRD"
+  by (rule NSRD_intro, simp_all add: closure unrest rdes)
+
+subsection \<open> State Abstraction \<close>
+
 definition state_srea ::
   "'s itself \<Rightarrow> ('s,'t::trace,'\<alpha>,'\<beta>) rel_rsp \<Rightarrow> (unit,'t,'\<alpha>,'\<beta>) rel_rsp" where
 [upred_defs]: "state_srea t P = \<langle>\<exists> {$st,$st\<acute>} \<bullet> P\<rangle>\<^sub>S"
@@ -27,19 +185,6 @@ syntax
 
 translations
   "state 'a \<bullet> P" == "CONST state_srea TYPE('a) P"
-
-lemma assigns_srd_RHS_tri_des [rdes_def]:
-  "\<langle>\<sigma>\<rangle>\<^sub>R = \<^bold>R\<^sub>s(true\<^sub>r \<turnstile> false \<diamondop> \<langle>\<sigma>\<rangle>\<^sub>r)"
-  by (rel_auto)
-
-lemma preR_assigns_srd [rdes]: "pre\<^sub>R(\<langle>\<sigma>\<rangle>\<^sub>R) = true\<^sub>r"
-  by (simp add: assigns_srd_def rea_pre_RHS_design usubst R2c_true)
-    
-lemma periR_assigns_srd [rdes]: "peri\<^sub>R(\<langle>\<sigma>\<rangle>\<^sub>R) = false"
-  by (simp add: assigns_srd_RHS_tri_des rea_peri_RHS_design usubst R2c_false R1_false)
-
-lemma postR_assigns_srd [rdes]: "post\<^sub>R(\<langle>\<sigma>\<rangle>\<^sub>R) = ($tr\<acute> =\<^sub>u $tr \<and> \<lceil>\<langle>\<sigma>\<rangle>\<^sub>a\<rceil>\<^sub>S \<and> $\<Sigma>\<^sub>S\<acute> =\<^sub>u $\<Sigma>\<^sub>S)"
-  apply (rel_auto) using minus_zero_eq by blast
 
 lemma R1_state_srea: "R1(state 'a \<bullet> P) = (state 'a \<bullet> R1(P))"
   by (rel_auto)
@@ -71,40 +216,197 @@ lemma periR_state_srea [rdes]: "peri\<^sub>R(state 'a \<bullet> P) = state 'a \<
 lemma postR_state_srea [rdes]: "post\<^sub>R(state 'a \<bullet> P) = state 'a \<bullet> post\<^sub>R(P)"
   by (rel_auto)
 
-lemma preR_choose [rdes]: "pre\<^sub>R(choose\<^sub>R) = true\<^sub>r"
-  by (rel_auto)
+subsection \<open> Iteration Construction \<close>
+  
+definition IterateR
+  :: "'a set \<Rightarrow> ('a \<Rightarrow> 's upred) \<Rightarrow> ('a \<Rightarrow> ('s, 't::trace, '\<alpha>) hrel_rsp) \<Rightarrow> ('s, 't, '\<alpha>) hrel_rsp"
+where "IterateR A g P = (\<mu>\<^sub>R X \<bullet> (if\<^sub>R i\<in>A \<bullet> g(i) \<rightarrow> P(i) fi ;; X) \<triangleleft> (\<Or> i\<in>A \<bullet> g(i)) \<triangleright>\<^sub>R II\<^sub>R)"
+   
+syntax
+  "_iter_srd" :: "pttrn \<Rightarrow> logic \<Rightarrow> logic \<Rightarrow> logic \<Rightarrow> logic" ("do\<^sub>R _\<in>_ \<bullet> _ \<rightarrow> _ fi")
+  
+translations
+  "_iter_srd x A g P" => "CONST IterateR A (\<lambda> x. g) (\<lambda> x. P)"
+  "_iter_srd x A g P" <= "CONST IterateR A (\<lambda> x. g) (\<lambda> x'. P)"
+  
+lemma IterateR_empty: 
+  "do\<^sub>R i\<in>{} \<bullet> g(i) \<rightarrow> P(i) fi = II\<^sub>R"
+  by (simp add: IterateR_def srd_mu_equiv closure rpred gfp_const)
 
-lemma periR_choose [rdes]: "peri\<^sub>R(choose\<^sub>R) = false"
-  by (rel_auto)
+subsection \<open> Substitution Laws \<close>
+  
+lemma srd_subst_Chaos [usubst]:
+  "\<sigma> \<dagger>\<^sub>S Chaos = Chaos"
+  by (rdes_simp)
 
-lemma postR_choose [rdes]: "post\<^sub>R(choose\<^sub>R) = true\<^sub>r"
-  by (rel_auto)
+lemma srd_subst_Miracle [usubst]:
+  "\<sigma> \<dagger>\<^sub>S Miracle = Miracle"
+  by (rdes_simp)
+
+lemma srd_subst_skip [usubst]:
+  "\<sigma> \<dagger>\<^sub>S II\<^sub>R = \<langle>\<sigma>\<rangle>\<^sub>R"
+  by (rdes_eq)
     
-lemma choose_srd_SRD [closure]: "choose\<^sub>R is SRD"
-  by (simp add: choose_srd_def closure unrest)
+lemma srd_subst_assigns [usubst]:
+  "\<sigma> \<dagger>\<^sub>S \<langle>\<rho>\<rangle>\<^sub>R = \<langle>\<rho> \<circ> \<sigma>\<rangle>\<^sub>R"
+  by (rdes_eq)
 
-lemma preR_cond_srea [rdes]:
-  "pre\<^sub>R(P \<triangleleft> b \<triangleright>\<^sub>R Q) = ([b]\<^sub>S\<^sub>< \<and> pre\<^sub>R(P) \<or> [\<not>b]\<^sub>S\<^sub>< \<and> pre\<^sub>R(Q))"
+subsection \<open> Algebraic Laws \<close>
+
+theorem assigns_srd_id: "\<langle>id\<rangle>\<^sub>R = II\<^sub>R"
+  by (rdes_eq)
+
+theorem assigns_srd_comp: "\<langle>\<sigma>\<rangle>\<^sub>R ;; \<langle>\<rho>\<rangle>\<^sub>R = \<langle>\<rho> \<circ> \<sigma>\<rangle>\<^sub>R"
+  by (rdes_eq)
+
+theorem assigns_srd_Miracle: "\<langle>\<sigma>\<rangle>\<^sub>R ;; Miracle = Miracle"
+  by (rdes_eq)
+
+theorem assigns_srd_Chaos: "\<langle>\<sigma>\<rangle>\<^sub>R ;; Chaos = Chaos"
+  by (rdes_eq)
+
+theorem assigns_srd_cond : "\<langle>\<sigma>\<rangle>\<^sub>R \<triangleleft> b \<triangleright>\<^sub>R \<langle>\<rho>\<rangle>\<^sub>R = \<langle>\<sigma> \<triangleleft> b \<triangleright>\<^sub>s \<rho>\<rangle>\<^sub>R"
+  by (rdes_eq)
+
+theorem assigns_srd_left_seq:
+  assumes "P is NSRD"
+  shows "\<langle>\<sigma>\<rangle>\<^sub>R ;; P = \<sigma> \<dagger>\<^sub>S P"
+  by (rdes_simp cls: assms)
+
+lemma AlternateR_empty: 
+  "if\<^sub>R i\<in>{} \<bullet> g(i) \<rightarrow> P(i) fi = Chaos"
+  by (simp add: AlternateR_def Chaos_def, rel_auto)
+
+lemma AlternateR_Chaos: 
+  "if\<^sub>R i\<in>A \<bullet> g(i) \<rightarrow> Chaos fi = Chaos"
+  by (simp add: AlternateR_def Chaos_def, rel_auto)
+
+lemma choose_srd_par:
+  "choose\<^sub>R \<parallel>\<^sub>R choose\<^sub>R = choose\<^sub>R"
+  by (rdes_eq)
+
+subsection \<open> Lifting designs to reactive designs \<close>
+
+definition des_rea_lift :: "'s hrel_des \<Rightarrow> ('s,'t::trace,'\<alpha>) hrel_rsp" ("\<^bold>R\<^sub>D") where
+[upred_defs]: "\<^bold>R\<^sub>D(P) = \<^bold>R\<^sub>s(\<lceil>pre\<^sub>D(P)\<rceil>\<^sub>S \<turnstile> (false \<diamondop> ($tr\<acute> =\<^sub>u $tr \<and> \<lceil>post\<^sub>D(P)\<rceil>\<^sub>S)))"
+
+definition des_rea_drop :: "('s,'t::trace,'\<alpha>) hrel_rsp \<Rightarrow> 's hrel_des" ("\<^bold>D\<^sub>R") where
+[upred_defs]: "\<^bold>D\<^sub>R(P) = \<lfloor>(pre\<^sub>R(P))\<lbrakk>$tr/$tr\<acute>\<rbrakk> \<restriction>\<^sub>v $st\<rfloor>\<^sub>S\<^sub><
+                     \<turnstile>\<^sub>n \<lfloor>(post\<^sub>R(P))\<lbrakk>$tr/$tr\<acute>\<rbrakk> \<restriction>\<^sub>v {$st,$st\<acute>}\<rfloor>\<^sub>S"
+
+lemma ndesign_rea_lift_inverse: "\<^bold>D\<^sub>R(\<^bold>R\<^sub>D(p \<turnstile>\<^sub>n Q)) = p \<turnstile>\<^sub>n Q"
+  apply (simp add: des_rea_lift_def des_rea_drop_def rea_pre_RHS_design rea_post_RHS_design)
+  apply (simp add: R1_def R2c_def R2s_def usubst unrest)
+  apply (rel_auto)
+  done
+
+lemma ndesign_rea_lift_injective:
+  assumes "P is \<^bold>N" "Q is \<^bold>N" "\<^bold>R\<^sub>D P = \<^bold>R\<^sub>D Q" (is "?RP(P) = ?RQ(Q)")
+  shows "P = Q"
+proof -
+  have "?RP(\<lfloor>pre\<^sub>D(P)\<rfloor>\<^sub>< \<turnstile>\<^sub>n post\<^sub>D(P)) = ?RQ(\<lfloor>pre\<^sub>D(Q)\<rfloor>\<^sub>< \<turnstile>\<^sub>n post\<^sub>D(Q))"
+    by (simp add: ndesign_form assms)
+  hence "\<lfloor>pre\<^sub>D(P)\<rfloor>\<^sub>< \<turnstile>\<^sub>n post\<^sub>D(P) = \<lfloor>pre\<^sub>D(Q)\<rfloor>\<^sub>< \<turnstile>\<^sub>n post\<^sub>D(Q)"
+    by (metis ndesign_rea_lift_inverse)
+  thus ?thesis
+    by (simp add: ndesign_form assms)
+qed
+        
+lemma des_rea_lift_closure [closure]: "\<^bold>R\<^sub>D(P) is SRD"
+  by (simp add: des_rea_lift_def RHS_design_is_SRD unrest)
+
+lemma preR_des_rea_lift [rdes]:
+  "pre\<^sub>R(\<^bold>R\<^sub>D(P)) = R1(\<lceil>pre\<^sub>D(P)\<rceil>\<^sub>S)"
   by (rel_auto)
 
-lemma periR_cond_srea [rdes]:
-  assumes "P is SRD" "Q is SRD"
-  shows "peri\<^sub>R(P \<triangleleft> b \<triangleright>\<^sub>R Q) = ([b]\<^sub>S\<^sub>< \<and> peri\<^sub>R(P) \<or> [\<not>b]\<^sub>S\<^sub>< \<and> peri\<^sub>R(Q))"
+lemma periR_des_rea_lift [rdes]:
+  "peri\<^sub>R(\<^bold>R\<^sub>D(P)) = (false \<triangleleft> \<lceil>pre\<^sub>D(P)\<rceil>\<^sub>S \<triangleright> ($tr \<le>\<^sub>u $tr\<acute>))"
+  by (rel_auto)
+
+lemma postR_des_rea_lift [rdes]:
+  "post\<^sub>R(\<^bold>R\<^sub>D(P)) = ((true \<triangleleft> \<lceil>pre\<^sub>D(P)\<rceil>\<^sub>S \<triangleright> (\<not> $tr \<le>\<^sub>u $tr\<acute>)) \<Rightarrow> ($tr\<acute> =\<^sub>u $tr \<and> \<lceil>post\<^sub>D(P)\<rceil>\<^sub>S))"
+  apply (rel_auto) using minus_zero_eq by blast
+
+lemma ndes_rea_lift_closure [closure]:
+  assumes "P is \<^bold>N"
+  shows "\<^bold>R\<^sub>D(P) is NSRD"
 proof -
-  have "peri\<^sub>R(P \<triangleleft> b \<triangleright>\<^sub>R Q) = peri\<^sub>R(R1(P) \<triangleleft> b \<triangleright>\<^sub>R R1(Q))"
-    by (simp add: Healthy_if SRD_healths assms)
-  thus ?thesis
-    by (rel_auto)
+  obtain p Q where P: "P = (p \<turnstile>\<^sub>n Q)"
+    by (metis H1_H3_commute H1_H3_is_normal_design H1_idem Healthy_def assms)
+  show ?thesis
+    apply (rule NSRD_intro)
+      apply (simp_all add: closure rdes unrest P)
+    apply (rel_auto)
+    done
 qed
 
-lemma postR_cond_srea [rdes]:
-  assumes "P is SRD" "Q is SRD"
-  shows "post\<^sub>R(P \<triangleleft> b \<triangleright>\<^sub>R Q) = ([b]\<^sub>S\<^sub>< \<and> post\<^sub>R(P) \<or> [\<not>b]\<^sub>S\<^sub>< \<and> post\<^sub>R(Q))"
+lemma R_D_mono:
+  assumes "P is \<^bold>H" "Q is \<^bold>H" "P \<sqsubseteq> Q"
+  shows "\<^bold>R\<^sub>D(P) \<sqsubseteq> \<^bold>R\<^sub>D(Q)"
+  apply (simp add: des_rea_lift_def)
+  apply (rule srdes_tri_refine_intro')
+    apply (auto intro: H1_H2_refines assms aext_mono)
+   apply (rel_auto)
+  apply (metis (no_types, hide_lams) aext_mono assms(3) design_post_choice
+      semilattice_sup_class.sup.orderE utp_pred_laws.inf.coboundedI1 utp_pred_laws.inf.commute utp_pred_laws.sup.order_iff)
+  done
+
+text {* Homomorphism laws *}
+
+lemma R_D_Miracle:
+  "\<^bold>R\<^sub>D(\<top>\<^sub>D) = Miracle"
+  by (simp add: Miracle_def, rel_auto)
+
+lemma R_D_Chaos:
+  "\<^bold>R\<^sub>D(\<bottom>\<^sub>D) = Chaos"
 proof -
-  have "post\<^sub>R(P \<triangleleft> b \<triangleright>\<^sub>R Q) = post\<^sub>R(R1(P) \<triangleleft> b \<triangleright>\<^sub>R R1(Q))"
-    by (simp add: Healthy_if SRD_healths assms)
-  thus ?thesis
+  have "\<^bold>R\<^sub>D(\<bottom>\<^sub>D) = \<^bold>R\<^sub>D(false \<turnstile>\<^sub>r true)"
     by (rel_auto)
+  also have "... = \<^bold>R\<^sub>s (false \<turnstile> false \<diamondop> ($tr\<acute> =\<^sub>u $tr))"
+    by (simp add: Chaos_def des_rea_lift_def alpha)
+  also have "... = \<^bold>R\<^sub>s (true)"
+    by (rel_auto)
+  also have "... = Chaos"
+    by (simp add: Chaos_def design_false_pre)
+  finally show ?thesis .
 qed
+
+lemma R_D_inf:
+  "\<^bold>R\<^sub>D(P \<sqinter> Q) = \<^bold>R\<^sub>D(P) \<sqinter> \<^bold>R\<^sub>D(Q)"
+  by (rule antisym, rel_auto+)
+
+lemma R_D_cond:
+  "\<^bold>R\<^sub>D(P \<triangleleft> \<lceil>b\<rceil>\<^sub>D\<^sub>< \<triangleright> Q) = \<^bold>R\<^sub>D(P) \<triangleleft> b \<triangleright>\<^sub>R \<^bold>R\<^sub>D(Q)"
+  by (rule antisym, rel_auto+)
+   
+lemma R_D_seq_ndesign:
+  "\<^bold>R\<^sub>D(p\<^sub>1 \<turnstile>\<^sub>n Q\<^sub>1) ;; \<^bold>R\<^sub>D(p\<^sub>2 \<turnstile>\<^sub>n Q\<^sub>2) = \<^bold>R\<^sub>D((p\<^sub>1 \<turnstile>\<^sub>n Q\<^sub>1) ;; (p\<^sub>2 \<turnstile>\<^sub>n Q\<^sub>2))"
+  apply (rule antisym)
+   apply (rule SRD_refine_intro)
+       apply (simp_all add: closure rdes ndesign_composition_wp)
+  using dual_order.trans apply (rel_blast)
+  using dual_order.trans apply (rel_blast)
+   apply (rel_auto)
+  apply (rule SRD_refine_intro)
+      apply (simp_all add: closure rdes ndesign_composition_wp)
+    apply (rel_auto)
+   apply (rel_auto)
+  apply (rel_auto)
+  done
+
+lemma R_D_seq:
+  assumes "P is \<^bold>N" "Q is \<^bold>N"
+  shows "\<^bold>R\<^sub>D(P) ;; \<^bold>R\<^sub>D(Q) = \<^bold>R\<^sub>D(P ;; Q)"
+  by (metis R_D_seq_ndesign assms ndesign_form)
+
+text {* Thes laws are applicable only when there is no further alphabet extension *}
+
+lemma R_D_skip:
+  "\<^bold>R\<^sub>D(II\<^sub>D) = (II\<^sub>R :: ('s,'t::trace,unit) hrel_rsp)"
+  apply (rel_auto) using minus_zero_eq by blast+
+  
+lemma R_D_assigns:
+  "\<^bold>R\<^sub>D(\<langle>\<sigma>\<rangle>\<^sub>D) = (\<langle>\<sigma>\<rangle>\<^sub>R :: ('s,'t::trace,unit) hrel_rsp)"
+  by (simp add: assigns_d_def des_rea_lift_def alpha assigns_srd_RHS_tri_des, rel_auto)
 
 end
