theories/rea_designs/utp_rdes_tactics.thy
@@ -1,0 +1,47 @@
+section {* Reactive design tactics *}
+
+theory utp_rdes_tactics
+  imports utp_rdes_triples
+begin
+
+text {* Tactic to expand out healthy reactive design predicates into the syntactic triple form. *}
+  
+method rdes_expand uses cls = (insert cls, (erule RD_elim)+)    
+
+text {* Tactic to simplify the definition of a reactive design *}
+  
+method rdes_simp uses cls =
+  ((rdes_expand cls: cls)?, (simp add: rdes_def rdes rpred cls closure alpha usubst unrest wp prod.case_eq_if))
+
+text {* Tactic to prove a refinement *}
+  
+method rdes_refine uses cls =
+  (rdes_simp cls: cls; rule_tac srdes_tri_refine_intro; (insert cls; rel_auto))
+
+text {* Tactics to prove an equality *}
+
+method rdes_eq uses cls =
+  (rdes_simp cls: cls; (rule_tac srdes_tri_eq_intro; insert cls; rel_auto))
+
+text {* Via antisymmetry *}
+
+method rdes_eq' uses cls =
+  (rdes_simp cls: cls; (rule_tac antisym; (rule_tac srdes_tri_refine_intro; insert cls; rel_auto)))
+
+text {* Tactic to calculate pre/peri/postconditions from reactive designs *}
+
+method rdes_calc = (simp add: rdes rpred closure alpha usubst unrest wp prod.case_eq_if)
+
+text {* The following tactic attempts to prove a reactive design refinement by calculation of
+  the pre-, peri-, and postconditions and then showing three implications between them using
+  rel_blast. *}
+
+method rdspl_refine =
+  (rule_tac SRD_refine_intro; (simp add: closure rdes unrest usubst ; rel_blast?))
+
+text {* The following tactic combines antisymmetry with the previous tactic to prove an equality. *}
+
+method rdspl_eq =
+  (rule_tac antisym, rdes_refine, rdes_refine)  
+
+end
