theories/rea_designs/utp_rea_designs.thy
@@ -1,0 +1,15 @@
+section \<open> Meta-theory for Reactive Designs \<close>
+
+theory utp_rea_designs
+  imports 
+    utp_rdes_healths
+    utp_rdes_designs
+    utp_rdes_triples
+    utp_rdes_normal
+    utp_rdes_contracts
+    utp_rdes_tactics
+    utp_rdes_parallel
+    utp_rdes_prog
+    utp_rdes_instant
+begin end
+
